130-145

src/lean4/human_eval/problem_122.lean
@@ -27,10 +27,11 @@ def problem_spec
 let spec (result: Int) :=
   1 ≤ arr.length → arr.length ≤ 100 → 1 ≤ k → k ≤ arr.length →
   ((∀ i, 0 ≤ i ∧ i < k → ¬(arr[i]! ≤ 99 ∧ -99 ≤ arr[i]!)) → result = 0) ∧
-  ∃ i, i < k ∧ arr[i]! ≤ 99 ∧ -99 ≤ arr[i]! →
-    result = arr[i]! + (if i = 0 then 0 else impl arr i) →
-  ∀ i', i < i' ∧ i' < k → ¬(arr[i']! ≤ 99 ∧ -99 ≤ arr[i']!)
--- program terminates
+  ∃ i, i < k
+    ∧ arr[i]! ≤ 99 ∧ -99 ≤ arr[i]!
+    ∧ result = arr[i]! + (if i = 0 then 0 else impl arr i)
+    ∧ ∀ i', i < i' ∧ i' < k → ¬(arr[i']! ≤ 99 ∧ -99 ≤ arr[i']!)
+-- program termination
 ∃ result, impl arr k = result ∧
 -- return value satisfies spec
 spec result
