src/lean4/human_eval/problem_131.lean
@@ -1,0 +1,83 @@
+import Imports.AllImports
+
+-- start_def problem_details
+/--
+function_signature: "def digits(n: int) -> int"
+docstring: |
+    Given a positive integer n, return the product of the odd digits.
+    Return 0 if all digits are even.
+test_cases:
+  - input: 1
+    expected_output: 1
+  - input: 4
+    expected_output: 0
+  - input: 235
+    expected_output: 15
+-/
+-- end_def problem_details
+
+-- start_def problem_spec
+def problem_spec
+-- function signature
+(impl: Int → Int)
+-- inputs
+(n: Int) :=
+-- spec
+let spec (result: Int) :=
+  0 < n →
+  (n < 10 → (n % 2 = 1 → result = n) ∧ (n % 2 = 0 → result = 0)) ∧
+  (10 ≤ n →
+    let digit := n % 10;
+    let rest := n / 10;
+    (digit % 2 = 1 → if impl rest = 0 then result = digit else result = impl rest * digit) ∧
+    (digit % 2 = 0 → result = impl rest))
+-- program termination
+∃ result, impl n = result ∧
+-- return value satisfies spec
+spec result
+-- end_def problem_spec
+
+-- start_def generated_spec
+def generated_spec
+-- function signature
+(impl: Int → Int)
+-- inputs
+(n: Int) : Prop :=
+-- end_def generated_spec
+--start_def generated_spec_body
+sorry
+--end_def generated_spec_body
+
+-- start_def spec_isomorphism
+theorem spec_isomorphism:
+∀ impl,
+(∀ n, problem_spec impl n) ↔
+(∀ n, generated_spec impl n) :=
+-- end_def spec_isomorphism
+-- start_def spec_isomorphism_proof
+sorry
+-- end_def spec_isomorphism_proof
+
+-- start_def implementation_signature
+def implementation (n: Int) : Int :=
+-- end_def implementation_signature
+-- start_def implementation
+sorry
+-- end_def implementation
+
+-- Uncomment the following test cases after implementing the function
+-- start_def test_cases
+-- #test implementation 1 = 1
+-- #test implementation 4 = 0
+-- #test implementation 235 = 15
+-- end_def test_cases
+
+
+-- start_def correctness_definition
+theorem correctness
+(n: Int)
+: problem_spec implementation n :=
+-- end_def correctness_definition
+-- start_def correctness_proof
+sorry
+-- end_def correctness_proof
