src/lean4/human_eval/problem_134.lean
@@ -1,0 +1,86 @@
+import Imports.AllImports
+
+-- start_def problem_details
+/--
+function_signature: "def check_if_last_char_is_a_letter(txt: String) -> Bool"
+docstring: |
+    Create a function that returns True if the last character
+    of a given string is an alphabetical character and is not
+    a part of a word, and False otherwise.
+    Note: "word" is a group of characters separated by space.
+test_cases:
+  - input: "apple pie"
+    expected_output: False
+  - input: "apple pi e"
+    expected_output: True
+  - input: "apple pi e "
+    expected_output: False
+  - input: ""
+    expected_output: False
+-/
+-- end_def problem_details
+
+-- start_def problem_spec
+def problem_spec
+-- function signature
+(impl: String → Bool)
+-- inputs
+(txt: String) :=
+-- spec
+let spec (result: Bool) :=
+  let words := txt.splitOn " ";
+  match words with
+  | [] => result = False
+  | [last_word] => (result ↔ last_word.length = 1) ∧ (let diff := (last_word.get 0).toLower.toNat - 'a'.toNat; 0 ≤ diff ∧ diff ≤ 25)
+  | head::tail => result ↔ (let tail_txt := String.join tail; impl tail_txt);
+-- program terminates
+∃ result, impl txt = result ∧
+-- return value satisfies spec
+spec result
+-- end_def problem_spec
+
+-- start_def generated_spec
+def generated_spec
+-- function signature
+(impl: String → Bool)
+-- inputs
+(txt: String) : Prop :=
+-- end_def generated_spec
+--start_def generated_spec_body
+sorry
+--end_def generated_spec_body
+
+-- start_def spec_isomorphism
+theorem spec_isomorphism:
+∀ impl,
+(∀ txt, problem_spec impl txt) ↔
+(∀ txt, generated_spec impl txt) :=
+-- end_def spec_isomorphism
+-- start_def spec_isomorphism_proof
+sorry
+-- end_def spec_isomorphism_proof
+
+-- start_def implementation_signature
+def implementation (txt: String) : Bool :=
+-- end_def implementation_signature
+-- start_def implementation
+sorry
+-- end_def implementation
+
+-- Uncomment the following test cases after implementing the function
+-- start_def test_cases
+-- #test implementation "apple pie" = false
+-- #test implementation "apple pi e" = true
+-- #test implementation "apple pi e " = false
+-- #test implementation "" = false
+-- end_def test_cases
+
+
+-- start_def correctness_definition
+theorem correctness
+(txt: String)
+: problem_spec implementation txt :=
+-- end_def correctness_definition
+-- start_def correctness_proof
+sorry
+-- end_def correctness_proof
