src/lean4/human_eval/problem_136.lean
@@ -1,0 +1,85 @@
+import Imports.AllImports
+
+-- start_def problem_details
+/--
+function_signature: "def largest_smallest_integers(lst: List[int]) -> Tuple[ Optional[Int], Optional[Int] ]"
+docstring: |
+    Create a function that returns a tuple (a, b), where 'a' is
+    the largest of negative integers, and 'b' is the smallest
+    of positive integers in a list.
+    If there is no negative or positive integers, return them as None.
+test_cases:
+  - input: [2, 4, 1, 3, 5, 7]
+    expected_output: (None, 1)
+  - input: []
+    expected_output: (None, None)
+  - input: [0]
+    expected_output: (None, None)
+-/
+-- end_def problem_details
+
+-- start_def problem_spec
+def problem_spec
+-- function signature
+(impl: List Int → Option Int × Option Int)
+-- inputs
+(lst: List Int) :=
+-- spec
+let spec (result: Option Int × Option Int) :=
+  let (a, b) := result;
+  (match a with
+  | none => ¬(∃ i, i ∈ lst ∧ i < 0)
+  | some a => a < 0 ∧ a ∈ lst ∧ ∀ i, i ∈ lst ∧ i < 0 → i ≤ a) ∧
+  (match b with
+  | none => ¬(∃ i, i ∈ lst ∧ 0 < i)
+  | some b => 0 < b ∧ b ∈ lst ∧ ∀ i, i ∈ lst ∧ 0 < i → b ≤ i)
+-- program termination
+∃ result, impl lst = result ∧
+-- return value satisfies spec
+spec result
+-- end_def problem_spec
+
+-- start_def generated_spec
+def generated_spec
+-- function signature
+(impl: List Int → Option Int × Option Int)
+-- inputs
+(lst: List Int) : Prop :=
+-- end_def generated_spec
+--start_def generated_spec_body
+sorry
+--end_def generated_spec_body
+
+-- start_def spec_isomorphism
+theorem spec_isomorphism:
+∀ impl,
+(∀ lst, problem_spec impl lst) ↔
+(∀ lst, generated_spec impl lst) :=
+-- end_def spec_isomorphism
+-- start_def spec_isomorphism_proof
+sorry
+-- end_def spec_isomorphism_proof
+
+-- start_def implementation_signature
+def implementation (lst: List Int) : (Option Int × Option Int) :=
+-- end_def implementation_signature
+-- start_def implementation
+sorry
+-- end_def implementation
+
+-- Uncomment the following test cases after implementing the function
+-- start_def test_cases
+-- #test implementation [2, 4, 1, 3, 5, 7] = (none, some 1)
+-- #test implementation [] = (none, none)
+-- #test implementation [0] = (none, none)
+-- end_def test_cases
+
+
+-- start_def correctness_definition
+theorem correctness
+(lst: List Int)
+: problem_spec implementation lst :=
+-- end_def correctness_definition
+-- start_def correctness_proof
+sorry
+-- end_def correctness_proof
