src/lean4/human_eval/problem_140.lean
@@ -1,0 +1,92 @@
+import Imports.AllImports
+
+-- start_def problem_details
+/--
+function_signature: "def fix_spaces(text: String) -> String"
+docstring: |
+    Given a string text, replace all spaces in it with underscores,
+    and if a string has more than 2 consecutive spaces,
+    then replace all consecutive spaces with -
+test_cases:
+  - input: "Example"
+    expected_output: "Example"
+  - input: "Example 1"
+    expected_output: "Example_1"
+  - input: " Example 2"
+    expected_output: "_Example_2"
+  - input: " Example   3"
+    expected_output: "_Example-3"
+-/
+-- end_def problem_details
+
+-- start_def problem_spec
+def problem_spec
+-- function signature
+(impl: String → String)
+-- inputs
+(text: String) :=
+-- spec
+let spec (result: String) :=
+  (result = "" → text = "") ∧
+  (result ≠ "" → (
+    (∃ pref s, text = pref ++ s
+      ∧ pref.length = 1
+      ∧ pref ≠ " "
+      ∧ result = pref ++ impl s)
+    ∨
+    (∃ pref s : String, text = pref ++ s ∧ pref ≠ "" ∧ (∀ ch, ch ∈ pref.toList → ch = ' ')
+      ∧ let k := pref.length;
+        (k ≤ 2 → result = (String.replicate k '_') ++ (impl (text.drop k)))
+      ∧ (2 < k → result = "-" ++ (impl (text.drop k)))) )
+  )
+-- program termination
+∃ result, impl text = result ∧
+-- return value satisfies spec
+spec result
+-- end_def problem_spec
+
+-- start_def generated_spec
+def generated_spec
+-- function signature
+(impl: String → String)
+-- inputs
+(text: String) : Prop :=
+-- end_def generated_spec
+--start_def generated_spec_body
+sorry
+--end_def generated_spec_body
+
+-- start_def spec_isomorphism
+theorem spec_isomorphism:
+∀ impl,
+(∀ text, problem_spec impl text) ↔
+(∀ text, generated_spec impl text) :=
+-- end_def spec_isomorphism
+-- start_def spec_isomorphism_proof
+sorry
+-- end_def spec_isomorphism_proof
+
+-- start_def implementation_signature
+def implementation (text: String) : String :=
+-- end_def implementation_signature
+-- start_def implementation
+sorry
+-- end_def implementation
+
+-- Uncomment the following test cases after implementing the function
+-- start_def test_cases
+-- #test implementation "Example" = "Example"
+-- #test implementation "Example 1" = "Example_1"
+-- #test implementation " Example 2" = "_Example_2"
+-- #test implementation " Example   3" = "_Example-3"
+-- end_def test_cases
+
+
+-- start_def correctness_definition
+theorem correctness
+(text: String)
+: problem_spec implementation text :=
+-- end_def correctness_definition
+-- start_def correctness_proof
+sorry
+-- end_def correctness_proof
