src/lean4/human_eval/problem_143.lean
@@ -1,0 +1,90 @@
+import Imports.AllImports
+
+-- start_def problem_details
+/--
+function_signature: "def words_in_sentence(sentence: String) -> String"
+docstring: |
+    You are given a string representing a sentence,
+    the sentence contains some words separated by a space,
+    and you have to return a string that contains the words from the original sentence,
+    whose lengths are prime numbers,
+    the order of the words in the new string should be the same as the original one.
+
+    Constraints:
+    * 1 <= len(sentence) <= 100
+    * sentence contains only letters
+test_cases:
+  - input: "This is a test"
+    expected_output: "is"
+  - input: "lets go for swimming"
+    expected_output: "go for"
+-/
+-- end_def problem_details
+
+-- start_def problem_spec
+def problem_spec
+-- function signature
+(impl: String → String)
+-- inputs
+(sentence: String) :=
+-- spec
+let spec (result: String) :=
+let words := sentence.splitOn;
+let result_words := result.splitOn;
+  1 ≤ sentence.length → sentence.length ≤ 100 →
+  sentence.all (fun x => let diff := x.toLower.toNat - 'a'.toNat; (0 ≤ diff ∧ diff ≤ 25) ∨ x = ' ') →
+  result_words.length ≤ words.length ∧
+  ∀ word ∈ result_words, word ∈ words ∧
+  match result_words with
+  | [] => ∀ word ∈ words, ¬(Nat.Prime word.length)
+  | head :: tail => if Nat.Prime head.length ∧ head = words[0]! then String.join tail = impl (String.join (words.drop 1))
+    else result = impl (String.join (words.drop 1))
+-- program termination
+∃ result, impl sentence = result ∧
+-- return value satisfies spec
+spec result
+-- end_def problem_spec
+
+-- start_def generated_spec
+def generated_spec
+-- function signature
+(impl: String → String)
+-- inputs
+(sentence: String) : Prop :=
+-- end_def generated_spec
+--start_def generated_spec_body
+sorry
+--end_def generated_spec_body
+
+-- start_def spec_isomorphism
+theorem spec_isomorphism:
+∀ impl,
+(∀ sentence, problem_spec impl sentence) ↔
+(∀ sentence, generated_spec impl sentence) :=
+-- end_def spec_isomorphism
+-- start_def spec_isomorphism_proof
+sorry
+-- end_def spec_isomorphism_proof
+
+-- start_def implementation_signature
+def implementation (sentence : String) : String :=
+-- end_def implementation_signature
+-- start_def implementation
+sorry
+-- end_def implementation
+
+-- Uncomment the following test cases after implementing the function
+-- start_def test_cases
+-- #test implementation "This is a test" = "is"
+-- #test implementation "lets go for swimming" = "go for"
+-- end_def test_cases
+
+
+-- start_def correctness_definition
+theorem correctness
+(sentence : String)
+: problem_spec implementation sentence :=
+-- end_def correctness_definition
+-- start_def correctness_proof
+sorry
+-- end_def correctness_proof
